kuiops/reduce/Kuiops.HReducePoly.Exact.fsti
@@ -12,26 +12,28 @@ module Kuiops.HReducePoly.Exact
 #lang-pulse
 
 open Kuiper
-open Kuiper.Seq.Common
 open Kuiper.Functions { is_associative }
-open Kuiper.Tensor { ctlayout }
+open Kuiper.Tensor
+open Kuiper.Seq.Common
 module SZ = Kuiper.SizeT
-module Array1 = Kuiper.Array1
 
 (* Non-empty left-to-right reduction ([foldl1]) of a sequence. *)
 let rfold1 (#et:Type0) (f : et -> et -> et) (s : seq et { Seq.length s > 0 })
   : GTot et
   = seq_fold_left f (s @! 0) (Seq.slice s 1 (Seq.length s))
 
+// TODO: should only need a fraction of a
+// TODO: support different accumulator type (need to supply another function to convert initial element)
+// This can be useful in the case of tracking both a sum and a max, for instance.
 inline_for_extraction noextract
 type reduce_ty (et : Type0) {| sized et |} =
   fn (f : (et -> et -> et) { is_associative f })
      (pre_map : et -> et)
      (nth : szp { nth <= max_threads })
      (lena : sz { SZ.fits (lena + nth) /\ SZ.v nth <= SZ.v lena })
-     (#l : Array1.layout lena) {| ctlayout l |}
-     (a : Array1.t et l { Array1.is_global a })
-     (#va : erased (lseq et lena))
+     (#l : layout1 lena) {| ctlayout l |}
+     (a : array1 et l { is_global a })
+     (#va : chest1 et lena)
   preserves
     cpu **
     on gpu_loc (a |-> va)
@@ -40,7 +42,7 @@ type reduce_ty (et : Type0) {| sized et |} =
   returns
     res : et
   ensures
-    pure (res == rfold1 f (lseq_map pre_map va))
+    pure (res == rfold1 f (lseq_map pre_map (chest1_to_seq va)))
 
 inline_for_extraction noextract
 val reduce (#et:Type0) {| sized et |} : reduce_ty et
